VerseRocq/verse/densem/env.v
@@ -47,3 +47,5 @@ Check  x |-> v, y |-> w.
 End NotationExamples.
 
 End EnvNotation.
+
+
