VerseRocq/verse/syntax/imports.v
@@ -1,4 +1,9 @@
 Require Import autosubst.lib autosubst.fintype.
 Require Export syntax.common.
-Require Import Setoid Morphisms Relation_Definitions.
+Require Export Setoid Morphisms Relation_Definitions.
+From Stdlib Require Export Program.Basics.
+From Stdlib Require Export Classes.EquivDec.
 
+From Stdlib Require Export Logic.PropExtensionality.
+From Stdlib Require Export Logic.FunctionalExtensionality.
+From Stdlib Require Export Sets.Classical_sets.
